STUFF DONE TODAY

AVL Tree.v
@@ -3,19 +3,20 @@ Require Export SfLib.
 Inductive tree: Type :=
 	| leaf : tree
 	| node : nat -> nat -> tree -> tree -> tree.
+	        (* Value -> Weight -> Left -> Right *)
 
 Check node 5 2 (node 3 0 leaf leaf) leaf.
 
 Definition left (t: tree) := 
 	match t with
-	| leaf => t
-	| node _ _ leftChild _ => leftChild
+	| leaf => None
+	| node _ _ leftChild _ => Some leftChild
 	end.
 
 Definition right (t: tree) := 
 	match t with
-	| leaf => t
-	| node _ _ _ rightChild => rightChild
+	| leaf => None
+	| node _ _ _ rightChild => Some rightChild
 	end.
 
 
@@ -25,15 +26,64 @@ Fixpoint height (t: tree) :=
 	| node _ _ leftChild rightChild => 1 + max (height leftChild) (height rightChild)
 	end.
 
-Definition insert (val:nat) (t: tree) := 
-	node val (height t) leaf t.
+
+Fixpoint insert (val:nat) (t: tree) := 
+	match t with
+	| leaf => node val 0 leaf leaf
+	| node treeval weight lChild rChild => match ble_nat val treeval with
+										   | true => node treeval (weight+1) (insert val lChild) rChild
+										   | false => node treeval (weight-1) lChild (insert val rChild)
+										   end
+	end.
+
+Example insertexample:
+	insert 2 (insert 5 leaf) = node 5 1 (node 2 0 leaf leaf) leaf.
+Proof. reflexivity. Qed.
+
+(*TODO: Look at weights *)
+Fixpoint balance (t : tree) :=
+	match t with
+	| leaf => leaf
+	| node val weight lChild rChild => 
+		match weight+2 with
+		| 0 => 
+			match rChild with
+			| leaf => leaf (* shouldn't happen *)
+			| node rval rweight rlChild rrChild => 
+				match rweight+2 with
+				| 1 => node rval (height (node val weight lChild rlChild) - height rrChild) (node val weight lChild rlChild) rrChild (* rr *)
+				| _ => 
+					match rlChild with
+						| leaf => leaf (* shouldn't happen*)
+						| node rlval rlweight rllChild rlrChild => 
+							node rlval 0 (node val weight lChild rllChild) (node rval 0 rlrChild rrChild) (* rl *)
+					end
+				end
+			end
+		| 4 => 
+			match lChild with
+			| leaf => leaf (* shouldn't happen *)
+			| node lval lweight llChild lrChild => 
+				match lweight+2 with
+				| 1 => 
+					match lrChild with
+					| leaf => leaf (* shouldn't happen *)
+					| node lrval lrweight lrlChild lrrChild => 
+						node lrval 0 (node lval 0 llChild lrlChild) (node val 0 lrrChild rChild) (* lr *)
+					end
+				| _ => node lval 0 llChild (node val 0 lrChild rChild) (* ll *)
+				end
+			end
+		| _ => node val weight (balance lChild) (balance rChild)
+		end
+	end.
 
 Example leftexample :
-	left (node 3 1 leaf (node 2 0 leaf leaf)) = leaf.
+	left (node 3 1 leaf (node 2 0 leaf leaf)) = Some leaf.
 Proof. reflexivity. Qed.
 
 Example rightexample :
-	right (node 3 1 (node 2 0 leaf leaf) leaf) = leaf.
+	right (node 3 1 (node 2 0 leaf leaf) leaf) = Some leaf.
 Proof. reflexivity. Qed.
 
 Example insertexample :
@@ -50,19 +100,22 @@ Proof. reflexivity. Qed.
 
 Fixpoint search (searchFor : nat) (t : tree) :=
 	match t with
-	| leaf => false
+	| leaf => None
 	| node val _ leftChild rightChild => match beq_nat val searchFor with
-										| true => true
-										| false => orb (search searchFor leftChild) (search searchFor rightChild)
+										| true => Some t
+										| false => match ble_nat searchFor val with
+												   | true => search searchFor leftChild
+												   | false => search searchFor rightChild
+												   end
 										end
 	end.
 
 Example searchexample :
-	search 5 (node 2 1 leaf (node 5 0 leaf leaf)) = true.
+	search 5 (node 2 1 leaf (node 5 0 leaf leaf)) = Some (node 5 0 leaf leaf).
 Proof. reflexivity. Qed.
 
 Example searchexample2 : 
-	search 5 leaf = false.
+	search 5 leaf = None.
 Proof. reflexivity. Qed.
 
 Fixpoint wellformed (t: tree) :=
@@ -87,34 +140,15 @@ Example inorder_test :
 	inorder Tree = 1::2::5::[].
 Proof. reflexivity. Qed.
 
-Fixpoint is_sorted (l : list nat) :=
-	match l with
-	| x1::xs => match xs with
-				| [] => true
-				| x2::xss => andb (ble_nat x1 x2) (is_sorted xs)
-				end
-	| [] => true
-	end.
-
-Example is_sortedexample :
-	is_sorted (inorder Tree) = true.
-Proof. reflexivity. Qed.
-
 Inductive sorted : list nat -> Prop :=
-	empty : sorted []
+	| empty : sorted []
 	| single : forall n, sorted [n]
 	| more : forall n m xs, ble_nat n m = true -> sorted (m::xs) -> sorted (n::m::xs).
 	
 Example propsorted :
 	sorted (inorder Tree).
-Proof. simpl. apply more. reflexivity. apply more. reflexivity. apply single. Qed.
+Proof. simpl. repeat apply more; try reflexivity. apply single. Qed.
 
 Example propnonsorted :
 	sorted (1::1::0::[]).
 Proof. apply more. reflexivity. apply more. (*UNPOSSIBLE!!!*) Admitted.
-
-Example hejmor : 
-	sorted [5].
-Proof.
-	apply single.
-Qed.
